%!TEX root = ../fro.tex
\chapter{Programmazione Lineare e Dualit√†}
\newcommand\scalemath[2]{\scalebox{#1}{\mbox{\ensuremath{\displaystyle #2}}}}

\Es
\begin{gather*}
\min 5x_{1} -2x_{2} -3x_{3}\\
-x_{1} +4x_{2} -2x_{3} +s_{1} =8\\
x_{1} +x_{2} +2x_{3} +s_{2} =12\\
x_{i} ,s_{i} \geq 0
\end{gather*}
\begin{equation*}
A=\begin{bmatrix}
x_{1} & x_{2} & x_{3} & s_{1} & s_{2}\\
-1 & 4 & -2 & 1 & 0\\
1 & 1 & 2 & 0 & 1
\end{bmatrix} \ \ b=\begin{bmatrix}
8\\
12
\end{bmatrix} \ \ c=\begin{bmatrix}
x_{1} & x_{2} & x_{3} & s_{1} & s_{2}\\
5 & -2 & -3 & 0 & 0
\end{bmatrix}
\end{equation*}

\begin{equation*}
\scalemath{0.65}{
\begin{array}{ c|c c c c c c c c c c c c c }
 & B & A_{B} & A_{B}^{-1} & c_{B}^{T} & c_{N}^{T} & A_{N} & A_{B}^{-1} A_{N} & r_{N}^{T} & x_{B} & \left( A_{B}^{-1} A_{N}\right)_{i} & \begin{bmatrix}
\vartheta _{1}\\
\vartheta _{2}
\end{bmatrix} & \text{IN} & \text{OUT}\\
\hline
\text{iter.} \ 1 & \{s_{1} ,s_{2}\} & \begin{bmatrix}
1 & 0\\
0 & 1
\end{bmatrix} & \begin{bmatrix}
1 & 0\\
0 & 1
\end{bmatrix} & \begin{bmatrix}
0 & 0
\end{bmatrix} & \begin{bmatrix}
5 & -2 & -3
\end{bmatrix} & \begin{bmatrix}
x_{1} & x_{2} & x_{3}\\
-1 & 4 & -2\\
1 & 1 & 2
\end{bmatrix} & \begin{bmatrix}
-1 & 4 & -2\\
1 & 1 & 2
\end{bmatrix} & \begin{bmatrix}
5 & -2 & -3
\end{bmatrix} & \begin{bmatrix}
8\\
12
\end{bmatrix} & \begin{bmatrix}
4\\
1
\end{bmatrix} & \begin{bmatrix}
2\\
12
\end{bmatrix} & x_{2} =2 & s_{1} =0\\
\text{iter.} \ 2 & \{x_{2} ,s_{2}\} & \begin{bmatrix}
4 & 0\\
1 & 1
\end{bmatrix} & \begin{bmatrix}
\frac{1}{4} & 0\\
-\frac{1}{4} & 1
\end{bmatrix} & \begin{bmatrix}
-2 & 0
\end{bmatrix} & \begin{bmatrix}
5 & -3 & 0
\end{bmatrix} & \begin{bmatrix}
x_{1} & x_{3} & s_{1}\\
-1 & -2 & 1\\
1 & 2 & 0
\end{bmatrix} & \begin{bmatrix}
-\frac{1}{4} & -\frac{1}{2} & \frac{1}{4}\\
\frac{5}{4} & \frac{5}{2} & -\frac{1}{4}
\end{bmatrix} & \begin{bmatrix}
\frac{9}{2} & -4 & \frac{1}{2}
\end{bmatrix} & \begin{bmatrix}
2\\
10
\end{bmatrix} & \begin{bmatrix}
-\frac{1}{2}\\
\frac{5}{2}
\end{bmatrix} & \begin{bmatrix}
-4\\
4
\end{bmatrix} & x_{3} =4 & s_{2} =0\\
\text{iter.} \ 3 & \{x_{2} ,x_{3}\} & \begin{bmatrix}
4 & -2\\
1 & 2
\end{bmatrix} & \begin{bmatrix}
\frac{1}{5} & \frac{1}{5}\\
-\frac{1}{10} & \frac{2}{5}
\end{bmatrix} & \begin{bmatrix}
-2 & -3
\end{bmatrix} & \begin{bmatrix}
5 & 0 & 0
\end{bmatrix} & \begin{bmatrix}
x_{1} & s_{1} & s_{2}\\
-1 & 1 & 0\\
1 & 0 & 1
\end{bmatrix} & \begin{bmatrix}
0 & \frac{1}{5} & \frac{1}{5}\\
\frac{1}{2} & -\frac{1}{10} & \frac{2}{5}
\end{bmatrix} & \begin{bmatrix}
\frac{13}{2} & \frac{1}{10} & \frac{7}{5}
\end{bmatrix} & \begin{bmatrix}
4\\
4
\end{bmatrix} &  &  &  & 
\end{array}
}
\end{equation*}
$z^{*} =-20$.

\Es
\begin{gather*}
\min -x_{1} +2x_{2} -3x_{3}\\
x_{1} -2x_{2} +x_{3} +s_{1} =2\\
3x_{1} -x_{2} +2x_{3} +s_{2} =6\\
x_{i} ,s_{i} \geq 0
\end{gather*}

\begin{equation*}
A=\begin{bmatrix}
x_{1} & x_{2} & x_{3} & s_{1} & s_{2}\\
1 & -2 & 1 & 1 & 0\\
3 & -1 & 2 & 0 & 1
\end{bmatrix} \ \ b=\begin{bmatrix}
2\\
6
\end{bmatrix} \ \ c=\begin{bmatrix}
x_{1} & x_{2} & x_{3} & s_{1} & s_{2}\\
-1 & 2 & -3 & 0 & 0
\end{bmatrix}
\end{equation*}

\begin{equation*}
\scalemath{0.65}{
\begin{array}{ c|c c c c c c c c c c c c c }
 & B & A_{B} & A_{B}^{-1} & c_{B}^{T} & c_{N}^{T} & A_{N} & A_{B}^{-1} A_{N} & r_{N}^{T} & x_{B} & \left( A_{B}^{-1} A_{N}\right)_{i} & \begin{bmatrix}
\vartheta _{1}\\
\vartheta _{2}
\end{bmatrix} & \text{IN} & \text{OUT}\\
\hline
\text{iter.} \ 1 & \{s_{1} ,s_{2}\} & \begin{bmatrix}
1 & 0\\
0 & 1
\end{bmatrix} & \begin{bmatrix}
1 & 0\\
0 & 1
\end{bmatrix} & \begin{bmatrix}
0 & 0
\end{bmatrix} & \begin{bmatrix}
-1 & 2 & -3
\end{bmatrix} & \begin{bmatrix}
x_{1} & x_{2} & x_{3}\\
1 & -2 & 1\\
3 & -1 & 2
\end{bmatrix} & \begin{bmatrix}
1 & -2 & 1\\
3 & -1 & 2
\end{bmatrix} & \begin{bmatrix}
-1 & 2 & -3
\end{bmatrix} & \begin{bmatrix}
2\\
6
\end{bmatrix} & \begin{bmatrix}
1\\
3
\end{bmatrix} & \begin{bmatrix}
1\\
2
\end{bmatrix} & x_{1} =2 & s_{1} =0\\
\text{iter.} \ 2 & \{x_{1} ,s_{2}\} & \begin{bmatrix}
1 & 0\\
3 & 1
\end{bmatrix} & \begin{bmatrix}
1 & 0\\
-3 & 1
\end{bmatrix} & \begin{bmatrix}
-1 & 0
\end{bmatrix} & \begin{bmatrix}
2 & -3 & 0
\end{bmatrix} & \begin{bmatrix}
x_{2} & x_{3} & s_{1}\\
-2 & 1 & 1\\
-1 & 2 & 0
\end{bmatrix} & \begin{bmatrix}
-2 & 1 & 1\\
5 & -1 & -3
\end{bmatrix} & \begin{bmatrix}
0 & -2 & 1
\end{bmatrix} & \begin{bmatrix}
2\\
0
\end{bmatrix} & \begin{bmatrix}
1\\
-1
\end{bmatrix} & \begin{bmatrix}
2\\
0
\end{bmatrix} & x_{3} =2 & x_{1} =0\\
\text{iter.} \ 3 & \{x_{3} ,s_{2}\} & \begin{bmatrix}
1 & 0\\
2 & 1
\end{bmatrix} & \begin{bmatrix}
1 & 0\\
-2 & 1
\end{bmatrix} & \begin{bmatrix}
-3 & 0
\end{bmatrix} & \begin{bmatrix}
-1 & 2 & 0
\end{bmatrix} & \begin{bmatrix}
x_{1} & x_{2} & s_{1}\\
1 & -2 & 1\\
3 & -1 & 0
\end{bmatrix} & \begin{bmatrix}
1 & -2 & 1\\
1 & 3 & -2
\end{bmatrix} & \begin{bmatrix}
2 & -4 & 3
\end{bmatrix} & \begin{bmatrix}
2\\
2
\end{bmatrix} & \begin{bmatrix}
-2\\
3
\end{bmatrix} & \begin{bmatrix}
-1\\
2/3
\end{bmatrix} & x_{2} =\frac{2}{3} & s_{2} =0\\
\text{iter.} \ 4 & \{x_{2} ,x_{3}\} & \begin{bmatrix}
-2 & 1\\
-1 & 2
\end{bmatrix} & \begin{bmatrix}
-\frac{2}{3} & \frac{1}{3}\\
-\frac{1}{3} & \frac{2}{3}
\end{bmatrix} & \begin{bmatrix}
2 & -3
\end{bmatrix} & \begin{bmatrix}
-1 & 0 & 0
\end{bmatrix} & \begin{bmatrix}
x_{1} & s_{1} & s_{2}\\
1 & 1 & 0\\
3 & 0 & 1
\end{bmatrix} & \begin{bmatrix}
\frac{1}{3} & -\frac{2}{3} & \frac{1}{3}\\
\frac{5}{3} & -\frac{1}{3} & \frac{2}{3}
\end{bmatrix} & \begin{bmatrix}
\frac{10}{3} & \frac{1}{3} & \frac{4}{3}
\end{bmatrix} & \begin{bmatrix}
\frac{2}{3}\\
\frac{10}{3}
\end{bmatrix} &  &  &  & 
\end{array}
}
\end{equation*}
$z^{*} =-\frac{26}{3}$.

\Es
\begin{gather*}
\min -2x_{1} -x_{2} -3x_{3}\\
x_{1} +x_{2} +x_{3} +s_{1} =2\\
2x_{1} +3x_{2} +8x_{3} +s_{2} =12\\
x_{i} ,s_{i} \geq 0
\end{gather*}
\begin{equation*}
A=\begin{bmatrix}
x_{1} & x_{2} & x_{3} & s_{1} & s_{2}\\
1 & 1 & 1 & 1 & 0\\
2 & 3 & 8 & 0 & 1
\end{bmatrix} \ \ b=\begin{bmatrix}
2\\
12
\end{bmatrix} \ \ c=\begin{bmatrix}
x_{1} & x_{2} & x_{3} & s_{1} & s_{2}\\
-2 & -1 & -3 & 0 & 0
\end{bmatrix}
\end{equation*}

\begin{equation*}
\scalemath{0.65}{
\begin{array}{ c|c c c c c c c c c c c c c }
 & B & A_{B} & A_{B}^{-1} & c_{B}^{T} & c_{N}^{T} & A_{N} & A_{B}^{-1} A_{N} & r_{N}^{T} & x_{B} & \left( A_{B}^{-1} A_{N}\right)_{i} & \begin{bmatrix}
\vartheta _{1}\\
\vartheta _{2}
\end{bmatrix} & \text{IN} & \text{OUT}\\
\hline
\text{iter.} \ 1 & \{s_{1} ,s_{2}\} & \begin{bmatrix}
1 & 0\\
0 & 1
\end{bmatrix} & \begin{bmatrix}
1 & 0\\
0 & 1
\end{bmatrix} & \begin{bmatrix}
0 & 0
\end{bmatrix} & \begin{bmatrix}
-2 & -1 & -3
\end{bmatrix} & \begin{bmatrix}
x_{1} & x_{2} & x_{3}\\
1 & 1 & 1\\
2 & 3 & 8
\end{bmatrix} & \begin{bmatrix}
1 & 1 & 1\\
2 & 3 & 8
\end{bmatrix} & \begin{bmatrix}
-2 & -1 & -3
\end{bmatrix} & \begin{bmatrix}
2\\
12
\end{bmatrix} & \begin{bmatrix}
1\\
2
\end{bmatrix} & \begin{bmatrix}
2\\
6
\end{bmatrix} & x_{1} =2 & s_{1} =0\\
\text{iter.} \ 2 & \{x_{1} ,s_{2}\} & \begin{bmatrix}
1 & 0\\
2 & 1
\end{bmatrix} & \begin{bmatrix}
1 & 0\\
-2 & 1
\end{bmatrix} & \begin{bmatrix}
-2 & 0
\end{bmatrix} & \begin{bmatrix}
-1 & -3 & 0
\end{bmatrix} & \begin{bmatrix}
x_{2} & x_{3} & s_{1}\\
1 & 1 & 1\\
3 & 8 & 0
\end{bmatrix} & \begin{bmatrix}
1 & 1 & 1\\
1 & 6 & -2
\end{bmatrix} & \begin{bmatrix}
1 & -1 & 2
\end{bmatrix} & \begin{bmatrix}
2\\
8
\end{bmatrix} & \begin{bmatrix}
1\\
6
\end{bmatrix} & \begin{bmatrix}
2\\
4/3
\end{bmatrix} & x_{3} =\frac{4}{3} & s_{2} =0\\
\text{iter.} \ 3 & \{x_{1} ,x_{3}\} & \begin{bmatrix}
1 & 1\\
2 & 8
\end{bmatrix} & \begin{bmatrix}
\frac{4}{3} & -\frac{1}{6}\\
-\frac{1}{3} & \frac{1}{6}
\end{bmatrix} & \begin{bmatrix}
-2 & -3
\end{bmatrix} & \begin{bmatrix}
-1 & 0 & 0
\end{bmatrix} & \begin{bmatrix}
x_{2} & s_{1} & s_{2}\\
1 & 1 & 0\\
3 & 0 & 1
\end{bmatrix} & \begin{bmatrix}
\frac{5}{6} & \frac{4}{3} & -\frac{1}{6}\\
\frac{1}{6} & -\frac{1}{3} & \frac{1}{6}
\end{bmatrix} & \begin{bmatrix}
\frac{7}{6} & \frac{5}{3} & \frac{1}{6}
\end{bmatrix} & \begin{bmatrix}
\frac{2}{3}\\
\frac{4}{3}
\end{bmatrix} &  &  &  & 
\end{array}
}
\end{equation*}
$z^{*} =\frac{16}{3}$.

\Es
\begin{gather*}
\min -2x_{1} +2x_{2} -2x_{3}\\
2x_{1} -2x_{2} -x_{3} +s_{1} =2\\
-3x_{1} +3x_{2} +2x_{3} +s_{2} =3\\
x_{i} ,s_{i} \geq 0
\end{gather*}
\begin{equation*}
A=\begin{bmatrix}
x_{1} & x_{2} & x_{3} & s_{1} & s_{2}\\
2 & -2 & -1 & 1 & 0\\
-3 & 3 & 2 & 0 & 1
\end{bmatrix} \ \ b=\begin{bmatrix}
2\\
3
\end{bmatrix} \ \ c=\begin{bmatrix}
x_{1} & x_{2} & x_{3} & s_{1} & s_{2}\\
-2 & 2 & -2 & 0 & 0
\end{bmatrix}
\end{equation*}

\begin{equation*}
\scalemath{0.65}{
\begin{array}{ c|c c c c c c c c c c c c c }
 & B & A_{B} & A_{B}^{-1} & c_{B}^{T} & c_{N}^{T} & A_{N} & A_{B}^{-1} A_{N} & r_{N}^{T} & x_{B} & \left( A_{B}^{-1} A_{N}\right)_{i} & \begin{bmatrix}
\vartheta _{1}\\
\vartheta _{2}
\end{bmatrix} & \text{IN} & \text{OUT}\\
\hline
\text{iter.} \ 1 & \{s_{1} ,s_{2}\} & \begin{bmatrix}
1 & 0\\
0 & 1
\end{bmatrix} & \begin{bmatrix}
1 & 0\\
0 & 1
\end{bmatrix} & \begin{bmatrix}
0 & 0
\end{bmatrix} & \begin{bmatrix}
-2 & 2 & -2
\end{bmatrix} & \begin{bmatrix}
x_{1} & x_{2} & x_{3}\\
2 & -2 & -1\\
-3 & 3 & 2
\end{bmatrix} & \begin{bmatrix}
2 & -2 & -1\\
-3 & 3 & 2
\end{bmatrix} & \begin{bmatrix}
-2 & 2 & -2
\end{bmatrix} & \begin{bmatrix}
2\\
3
\end{bmatrix} & \begin{bmatrix}
2\\
-3
\end{bmatrix} & \begin{bmatrix}
1\\
-1
\end{bmatrix} & x_{1} =2 & s_{1} =0\\
\text{iter.} \ 2 & \{x_{1} ,s_{2}\} & \begin{bmatrix}
2 & 0\\
-3 & 1
\end{bmatrix} & \begin{bmatrix}
\frac{1}{2} & 0\\
\frac{3}{2} & 1
\end{bmatrix} & \begin{bmatrix}
-2 & 0
\end{bmatrix} & \begin{bmatrix}
2 & -2 & 0
\end{bmatrix} & \begin{bmatrix}
x_{2} & x_{3} & s_{1}\\
-2 & -1 & 1\\
3 & 2 & 0
\end{bmatrix} & \begin{bmatrix}
-1 & -\frac{1}{2} & \frac{1}{2}\\
0 & \frac{1}{2} & \frac{3}{2}
\end{bmatrix} & \begin{bmatrix}
0 & -3 & 1
\end{bmatrix} & \begin{bmatrix}
1\\
6
\end{bmatrix} & \begin{bmatrix}
-\frac{1}{2}\\
\frac{1}{2}
\end{bmatrix} & \begin{bmatrix}
-\frac{1}{2}\\
12
\end{bmatrix} & x_{3} =12 & s_{2} =0\\
\text{iter.} \ 3 & \{x_{1} ,x_{3}\} & \begin{bmatrix}
2 & -1\\
-3 & 2
\end{bmatrix} & \begin{bmatrix}
2 & 1\\
3 & 2
\end{bmatrix} & \begin{bmatrix}
-2 & -2
\end{bmatrix} & \begin{bmatrix}
2 & 0 & 0
\end{bmatrix} & \begin{bmatrix}
x_{2} & s_{1} & s_{2}\\
-2 & 1 & 0\\
3 & 0 & 1
\end{bmatrix} & \begin{bmatrix}
-1 & 2 & 1\\
0 & 3 & 2
\end{bmatrix} & \begin{bmatrix}
12 & 10 & 6
\end{bmatrix} & \begin{bmatrix}
7\\
12
\end{bmatrix} &  &  &  & 
\end{array}
}
\end{equation*}
$z^{*} =-38$.

\Es
\begin{gather*}
\min x_{1} -2x_{2} +x_{3}\\
x_{1} -x_{2} +3x_{3} =5\\
2x_{1} +x_{2} +x_{3} =4\\
x_{i} \geq 0
\end{gather*}
Fase $1$.
\begin{gather*}
\min w_{1} +w_{2}\\
x_{1} -x_{2} +3x_{3} +w_{1} =5\\
2x_{1} +x_{2} +x_{3} +w_{2} =4\\
x_{i} \geq 0
\end{gather*}
\begin{equation*}
A=\begin{bmatrix}
x_{1} & x_{2} & x_{3} & w_{1} & w_{2}\\
1 & -1 & 3 & 1 & 0\\
2 & 1 & 1 & 0 & 1
\end{bmatrix} \ \ b=\begin{bmatrix}
5\\
4
\end{bmatrix} \ \ c=\begin{bmatrix}
x_{1} & x_{2} & x_{3} & w_{1} & w_{2}\\
0 & 0 & 0 & 1 & 1
\end{bmatrix}
\end{equation*}
\begin{equation*}
\scalemath{0.65}{
\begin{array}{ c|c c c c c c c c c c c c c }
 & B & A_{B} & A_{B}^{-1} & c_{B}^{T} & c_{N}^{T} & A_{N} & A_{B}^{-1} A_{N} & r_{N}^{T} & x_{B} & \left( A_{B}^{-1} A_{N}\right)_{i} & \begin{bmatrix}
\vartheta _{1}\\
\vartheta _{2}
\end{bmatrix} & \text{IN} & \text{OUT}\\
\hline
\text{iter.} \ 1 & \{w_{1} ,w_{2}\} & \begin{bmatrix}
1 & 0\\
0 & 1
\end{bmatrix} & \begin{bmatrix}
1 & 0\\
0 & 1
\end{bmatrix} & \begin{bmatrix}
1 & 1
\end{bmatrix} & \begin{bmatrix}
0 & 0 & 0
\end{bmatrix} & \begin{bmatrix}
x_{1} & x_{2} & x_{3}\\
1 & -1 & 3\\
2 & 1 & 1
\end{bmatrix} & \begin{bmatrix}
1 & -1 & 3\\
2 & 1 & 1
\end{bmatrix} & \begin{bmatrix}
-3 & 0 & -4
\end{bmatrix} & \begin{bmatrix}
5\\
4
\end{bmatrix} & \begin{bmatrix}
1\\
2
\end{bmatrix} & \begin{bmatrix}
5\\
2
\end{bmatrix} & x_{1} =2 & w_{2} =0\\
\text{iter.} \ 2 & \{x_{1} ,w_{1}\} & \begin{bmatrix}
1 & 1\\
2 & 0
\end{bmatrix} & \begin{bmatrix}
0 & \frac{1}{2}\\
1 & -\frac{1}{2}
\end{bmatrix} & \begin{bmatrix}
0 & 1
\end{bmatrix} & \begin{bmatrix}
0 & 0 & 1
\end{bmatrix} & \begin{bmatrix}
x_{2} & x_{3} & w_{2}\\
-1 & 3 & 0\\
1 & 1 & 1
\end{bmatrix} & \begin{bmatrix}
\frac{1}{2} & \frac{1}{2} & \frac{1}{2}\\
-\frac{3}{2} & \frac{5}{2} & -\frac{1}{2}
\end{bmatrix} & \begin{bmatrix}
\frac{3}{2} & -\frac{5}{2} & \frac{3}{2}
\end{bmatrix} & \begin{bmatrix}
2\\
3
\end{bmatrix} & \begin{bmatrix}
\frac{1}{2}\\
\frac{5}{2}
\end{bmatrix} & \begin{bmatrix}
4\\
\frac{6}{5}
\end{bmatrix} & x_{3} =\frac{6}{5} & w_{1} =0
\end{array}
}
\end{equation*}
Inizio.
\begin{equation*}
A=\begin{bmatrix}
x_{1} & x_{2} & x_{3}\\
1 & -1 & 3\\
2 & 1 & 1
\end{bmatrix} \ \ b=\begin{bmatrix}
5\\
4
\end{bmatrix} \ \ c=\begin{bmatrix}
x_{1} & x_{2} & x_{3}\\
1 & -2 & 1
\end{bmatrix}
\end{equation*}
\begin{equation*}
\scalemath{0.75}{
\begin{array}{ c|c c c c c c c c c c c c c }
 & B & A_{B} & A_{B}^{-1} & c_{B}^{T} & c_{N}^{T} & A_{N} & A_{B}^{-1} A_{N} & r_{N}^{T} & x_{B} & \left( A_{B}^{-1} A_{N}\right)_{i} & \begin{bmatrix}
\vartheta _{1}\\
\vartheta _{2}
\end{bmatrix} & \text{IN} & \text{OUT}\\
\hline
\text{iter.} \ 1 & \{x_{1} ,x_{3}\} & \begin{bmatrix}
1 & 3\\
2 & 1
\end{bmatrix} & \begin{bmatrix}
-\frac{1}{5} & \frac{3}{5}\\
\frac{2}{5} & -\frac{1}{5}
\end{bmatrix} & \begin{bmatrix}
1 & 1
\end{bmatrix} & \begin{bmatrix}
-2
\end{bmatrix} & \begin{bmatrix}
x_{2}\\
-1\\
1
\end{bmatrix} & \begin{bmatrix}
\frac{4}{5}\\
-\frac{3}{5}
\end{bmatrix} & \begin{bmatrix}
-\frac{11}{5}
\end{bmatrix} & \begin{bmatrix}
\frac{7}{5}\\
\frac{6}{5}
\end{bmatrix} & \begin{bmatrix}
\frac{4}{5}\\
-\frac{3}{5}
\end{bmatrix} & \begin{bmatrix}
\frac{7}{4}\\
-2
\end{bmatrix} & x_{2} =\frac{7}{4} & x_{1} =0\\
\text{iter.} \ 2 & \{x_{2} ,x_{3}\} & \begin{bmatrix}
-1 & 3\\
1 & 1
\end{bmatrix} & \begin{bmatrix}
-\frac{1}{4} & \frac{3}{4}\\
\frac{1}{4} & \frac{1}{4}
\end{bmatrix} & \begin{bmatrix}
-2 & 1
\end{bmatrix} & \begin{bmatrix}
1
\end{bmatrix} & \begin{bmatrix}
x_{1}\\
1\\
2
\end{bmatrix} & \begin{bmatrix}
\frac{5}{4}\\
\frac{3}{4}
\end{bmatrix} & \begin{bmatrix}
\frac{11}{4}
\end{bmatrix} & \begin{bmatrix}
\frac{7}{4}\\
\frac{9}{4}
\end{bmatrix} &  &  &  & 
\end{array}
}
\end{equation*}
$z^{*} =-\frac{5}{4}$.














\Es
Troppa fatica.
\Es
Troppa fatica.
\Es
Troppa fatica.



\Es

Problema duale.
\begin{gather*}
\min -y_{1} +y_{2} +17y_{3} +5y_{4} +4y_{5}\\
\begin{aligned}
-2y_{1} +y_{2} +4y_{3} -5y_{5} & \geq 2\\
-y_{1} -y_{2} +y_{3} +y_{4} +y_{5} & \geq 1\\
y_{i} & \geq 0
\end{aligned}
\end{gather*}
Scarti complementari.
\begin{equation*}
\begin{array}{ l|l|l }
 & ( 3,5) & ( 4,1)\\
\hline
( -2x_{1} -x_{2} +1) y_{1} =0 & y_{1} =0 & \\
( x_{1} -x_{2} -3) y_{2} =0 & y_{2} =0 & \\
( 4x_{1} +x_{2} -17) y_{3} =0 & y_{3} & \\
( x_{2} -5) y_{4} =0 & y_{4} & \\
( -x_{1} -x_{2} -4) y_{5} =0 & y_{5} =0 & \\
( -2y_{1} +y_{2} +4y_{3} -5y_{5} -2) x_{1} =0 & y_{3} =1/2 & \\
( -y_{1} -y_{2} +y_{3} +y_{4} +y_{5} -1) x_{2} =0 & y_{4} =1/2 & \\
\hline
 & \text{Ottimo} & \text{Non ottimo}
\end{array}
\end{equation*}
\Es

Problema duale.
\begin{gather*}
\min -\frac{3}{2} y_{1} -\frac{3}{2} y_{2} +7y_{3} +6y_{4}\\
\begin{aligned}
y_{1} +y_{3} +y_{4} & =3\\
y_{2} +y_{3} -y_{4} & =0\\
y_{1} ,y_{2} \leq 0,y_{3} ,y_{4} & \geq 0
\end{aligned}
\end{gather*}
Scarti complementari.
\begin{equation*}
\begin{array}{ l|l|l }
 & \left(\frac{13}{2} ,\frac{1}{2}\right) & \left( -\frac{3}{2} ,\frac{17}{2}\right)\\
\hline
\left( x_{1} +\frac{3}{2}\right) y_{1} =0 & y_{1} =0 & y_{1}\\
\left( x_{2} +\frac{3}{2}\right) y_{2} =0 & y_{2} =0 & y_{2} =0\\
( x_{1} +x_{2} -7) y_{3} =0 & y_{3} & y_{3}\\
( x_{1} -x_{2} -6) y_{4} =0 & y_{4} & y_{4} =0\\
( y_{1} +y_{3} +y_{4} -3) x_{1} =0 & y_{3} +y_{4} =3 & y_{1} +y_{3} =3\\
( y_{2} +y_{3} -y_{4}) x_{2} =0 & y_{3} -y_{4} =0 & y_{3} =0\\
\hline
 & y_{3} =3/2 & y_{1} =3\\
 & y_{4} =3/2 & \\
\hline
 & \text{Ottimo} & \text{Non ottimo}
\end{array}
\end{equation*}
\Es

Problema duale.
\begin{gather*}
\min 4y_{1} +5y_{2} +y_{3} +4y_{4}\\
\begin{aligned}
-3y_{1} +y_{3} +2y_{4} & =1\\
y_{1} +y_{2} -y_{3} +y_{4} & =2\\
y_{1} ,y_{2} ,y_{3} \geq 0,y_{4} & \leq 0
\end{aligned}
\end{gather*}
Scarti complementari.
\begin{equation*}
\begin{array}{ l|l|l }
 & ( 6,5) & ( 0,4)\\
\hline
( -3x_{1} +x_{2} -4) y_{1} =0 & y_{1} =0 & y_{1}\\
( x_{2} -5) y_{2} =0 & y_{2} & y_{2} =0\\
( x_{1} -x_{2} -1) y_{3} =0 & y_{3} & y_{3} =0\\
( 2x_{1} +x_{2} -4) y_{4} =0 & y_{4} =0 & y_{4}\\
( -3y_{1} +y_{3} +2y_{4} -1) x_{1} =0 & y_{3} =1 & -3y_{1} +2y_{4} =1\\
( y_{1} +y_{2} -y_{3} +y_{4} -2) x_{2} =0 & y_{2} =3 & y_{1} +y_{4} =2\\
\hline
 &  & y_{1} =3/5\\
 &  & y_{4} =7/5\\
\hline
 & \text{Ottimo} & \text{Non ottimo}
\end{array}
\end{equation*}